---
title: "Derivation of Computation of Empirical Variance"
output: html_notebook
---

The empirical variance is computed as

$$s^2 = {1 \over n-1}\sum_{i=1}^n (x_i - \mu)^2
=
 {1 \over n-1}\sum_{i=1}^n (x_i^2 - 2 \mu x_i + \mu^2)
=
 {1 \over n-1}\left[\sum_{i=1}^n x_i^2 - 2\mu \sum_{i=1}^n x_i + n*\mu^2 \right]
= 
{1 \over n-1}\left[\sum_{i=1}^n x_i^2 - 2n \mu^2 + n \mu^2 \right]
= 
{1 \over n-1}\left[\sum_{i=1}^n x_i^2 - n \mu^2 \right]
$$

where $\mu$ is a constant corresponding to 

$$\mu = {1 \over n}\sum_{i=1}^n x_i$$

Inserting $\mu$ back

$$
s^2 = {1 \over n-1}\left[\sum_{i=1}^n x_i^2 - n ({1 \over n}\sum_{i=1}^n x_i)^2 \right]
=
{1 \over n-1}\left[\sum_{i=1}^n x_i^2 - {1 \over n}(\sum_{i=1}^n x_i)^2 \right]
$$

